# Exercise
* **NOTE:** I messed up a 2 or 1/2 factor up somewhere, I think the z substitution should not have the $\sqrt{2}$ factor with the way I did it.
Recall that the normal distribution is defined by
$$
\mathcal{N}(x | \mu, \sigma^2) = \frac{1}{(2 \pi \sigma^2)^{1/2}}\exp\left( - \frac{1}{2\sigma^2} (x - \mu)^2 \right)
$$
where $\mu$ is called the mean and $\sigma^2$ the variance.

Also it is straightforward to show that the Gaussian is normalized, so that
$$
\int_{-\infty}^\infty \mathcal{N}(x | \mu, \sigma^2) dx = 1.
$$

# Solution
Let $z := \frac{x - \mu}{\sqrt{2} \sigma}$ then
$$
dz = \frac{1}{\sqrt{2}\sigma} dx
$$
i.e.
$$
dx = \sqrt{2}\sigma dz
$$
Note that $x = \pm \infty \implies z = \pm \infty$, with that we can write
$$
\begin{aligned}
\int_{-\infty}^\infty \mathcal{N}(x | \mu, \sigma^2) dx &= \int_{-\infty}^\infty \frac{1}{(2 \pi \sigma^2)^{1/2}}\exp\left( - \frac{1}{2\sigma^2} (x - \mu)^2 \right) dx \\
&= \frac{1}{(2 \pi \sigma^2)^{1 / 2}} \int_{-\infty}^\infty \exp\left( - \frac{1}{2\sigma^2} (x - \mu)^2 \right) dx \\
&= \frac{1}{(2 \pi \sigma^2)^{1 / 2}} \int_{-\infty}^\infty \exp\left( -z^2 \right) \sqrt{2}\sigma dz \\
&= \pi^{-1/2} \int_{-\infty}^\infty \exp\left(-z^2\right) dz
\end{aligned}
$$
As such it suffices to show that integrating $e^{-z^2}$ results in $\sqrt{\pi}$.

I won't fill in the remaining details, but the statement can be proven by noting that this function is symmetrical, so we can just double the integral from $0$ to $\infty$ and interpret this as the radius $r^2 = x^2 + y^2$ of the radially symmetrical function
$$
e^{-(x^2 + y^2)}
$$
and note that
$$
e^{-(x^2 + y^2)} = e^{-x^2}e^{-y^2}
$$
as such the integral over this whole thing is our desired integral squared. It's possible to show that the whole integral evaluates to $\pi$ and with that we are done.