# Exercise
$$
\begin{pmatrix}
A & B \\
C & D
\end{pmatrix}^{-1}
=
\begin{pmatrix}
M & -MBD^{-1} \\
-D^{-1}CM & D^{-1} + D^{-1}CMBD^{-1}
\end{pmatrix}
$$
where
$$
M = (A - BD^{-1}C)^{-1}.
$$
The quantity $M^{-1}$ is known as the Schur complement of the matrix on the left-hand side with respect to the submatrix $D$.

# Solution
It suffices to show that
$$
\begin{pmatrix}
M & -MBD^{-1} \\
-D^{-1}CM & D^{-1} + D^{-1}CMBD^{-1}
\end{pmatrix} \cdot \begin{pmatrix}
A & B \\
C & D
\end{pmatrix} = I.
$$
We can multiply this out and have to show that the following four identites hold:
$$
\begin{aligned}
I &= MA - MBD^{-1}C\\
0 &= MB - MBD^{-1}D \\
0 &= -D^{-1}CMA + D^{-1}A + D^{-1}CMBD^{-1}C \\
I &= -D^{-1}CMB + D^{-1}D + D^{-1} CMBD^{-1}D
\end{aligned}
$$

For the first equation we can factor out $M$ and the collected term is exactly the Schur complement:
$$
M\underbrace{(A - BD^{-1}C)}_{= M^{-1}} = I
$$
For the second equation we get
$$
M(B - BD^{-1}D) = M(B - B) = 0
$$
For the third we get
$$
D^{-1}(-CMA + C + CMBD^{-1}C) = D^{-1}(-CM(A - BD^{-1}C) + C) = D^{-1}(C - C) = 0
$$
And for the fourth we get
$$
-D^{-1}CMB + I + D^{-1}CMB = D^{-1}(CMB - CMB) + I = I.
$$