# Exercise
and so the Gaussian distribution over $\mathbf{z}$ has precision (inverse covariance) matrix
given by
$$
\mathbf{R} = \begin{pmatrix}
\mathbf{\Lambda} + \mathbf{A}^{\top} \mathbf{L} \mathbf{A} & - \mathbf{A}^{\top} \mathbf{L} \\
- \mathbf{L} \mathbf{A} & \mathbf{L}
\end{pmatrix}.
$$
The covariance matrix is found by taking the inverse of the precision, which can be done using the matrix inversion formula (2.76) to give
$$
\text{cov}[\mathbf{z}] = \mathbf{R}^{-1} = \begin{pmatrix}
\mathbf{\Lambda}^{-1} & \mathbf{\Lambda}^{-1} \mathbf{A}^{\top} \\
\mathbf{A} \mathbf{\Lambda}^{-1} & \mathbf{L}^{-1} + \mathbf{A} \mathbf{\Lambda}^{-1} \mathbf{A}^{\top}
\end{pmatrix}.
$$

# Solution
Recall 
$$
\begin{pmatrix}
\mathbf{A} & \mathbf{B} \\
\mathbf{C} & \mathbf{D}
\end{pmatrix}^{-1}
=
\begin{pmatrix}
\mathbf{M} & -\mathbf{M} \mathbf{B} \mathbf{D}^{-1} \\
-\mathbf{D}^{-1} \mathbf{C} \mathbf{M} & \mathbf{D}^{-1} + \mathbf{D}^{-1} \mathbf{C} \mathbf{M} \mathbf{B} \mathbf{D}^{-1}
\end{pmatrix}
$$
where we have defined
$$
\mathbf{M} = \left( \mathbf{A} - \mathbf{B} \mathbf{D}^{-1} \mathbf{C} \right)^{-1}.
$$

We can write R using
$$
\begin{aligned}
\alpha &= \Lambda + A^TLA \\
\beta &= -A^TL \\
\gamma &= -LA \\
\delta &= L
\end{aligned}
$$
as
$$
R = \begin{pmatrix} \alpha & \beta \\ \gamma & \delta \end{pmatrix}
$$
and define
$$
M := (\alpha - \beta \delta^{-1}\gamma)^{-1}
$$
and see that
$$
\begin{aligned}
\alpha - \beta \delta^{-1}\gamma &= (\Lambda + A^TLA) - (-A^TL) (L^{-1}) (-LA) \\
&= (\Lambda + A^TLA) - A^TLA = \Lambda
\end{aligned}
$$
holds, as such $M = \Lambda^{-1}$. With that we can see that
$$
R^{-1} =
\begin{pmatrix}
\Lambda^{-1} & -\Lambda^{-1}\beta\delta^{-1} \\ 
-\delta^{-1} \gamma \Lambda^{-1} & \delta^{-1} + \delta^{-1} \gamma \Lambda^{-1} \beta \delta^{-1}
\end{pmatrix}.
$$
We now compute the remaining entries
$$
\begin{aligned}
-\Lambda^{-1}\beta \delta^{-1} &= - \Lambda^{-1}(-A^TL)L^{-1} \\
&= \Lambda^{-1}A^T, \\
-\delta^{-1} \gamma \Lambda^{-1} &= -L^{-1} (-LA) \Lambda^{-1} \\
&= A\Lambda^{-1}, \\
\delta^{-1} + \delta^{-1} \gamma \Lambda^{-1} \beta \delta^{-1} &= L^{-1} + L^{-1} (-LA) \Lambda^{-1} (-A^TL) L^{-1} \\
&= L^{-1} + A\Lambda^{-1}A^T.\\
\end{aligned}
$$
As such the inverse of $R$ indeed has the desired form.