# Exercise
Show that the logistic sigmoid function (4.59) satisfies the property
$$
\sigma(-a) = 1 - \sigma(a)
$$
and that its inverse is given by
$$
\sigma^{-1}(y) = \log\left(\frac{y}{1 - y}\right).
$$

# Solution
Recall that
$$
\sigma(a) = \frac{1}{1 + \exp(-a)}.
$$
To see the first identity we note that $\exp(a)\exp(-a) = \exp(a - a) = \exp(0) = 1$ and compute
$$
\begin{aligned}
\sigma(a) + \sigma(-a) &= \frac{1}{1 + \exp(-a)} + \frac{1}{1 + \exp(a)} \\
&= \frac{(1 + \exp(a)) + (1 + \exp(-a))}{(1 + \exp(-a))(1 + \exp(a))} \\
&= \frac{2 + \exp(a) + \exp(-a)}{1 + \exp(a) + \exp(-a) + \exp(a)\exp(-a)} \\
&= 1.
\end{aligned}
$$

For the second identiy we compute
$$
\begin{aligned}
&&y &= \frac{1}{1 + \exp(-a)} \\
\iff&& y(1 + \exp(-a)) &= 1 \\
\iff&& \exp(-a) &= \frac{1}{y} - 1 \\
\iff&& \exp(-a) &= \frac{1 - y}{y} \\
\iff&& -a &= \log\left(\frac{1 - y}{y}\right) \\
\iff&& a &= \log\left(\frac{y}{1 - y}\right).
\end{aligned}
$$