# Exercise 5.29
Verify the result (5.141)

## Solution
This bascially reduces down to showing that
$$
\frac{\partial \Omega}{\partial w_i} = \sum_j \gamma_j(w_i) \frac{w_i - \mu_j}{\sigma_j^2}
$$
where
$$
\gamma_j(w) = \frac{\pi_j \mathcal{N}(w | \mu_j, \sigma_j^2)}{\sum_k \pi_k \mathcal{N}(w | \mu_k, \sigma_k^2)}
$$
We can write
$$
\zeta := \sum_k \pi_k \mathcal{N}(w | \mu_k, \sigma_k^2)
$$
to simplify
$$
\gamma_j(w) = \frac{\pi_j \mathcal{N}(w | \mu_j, \sigma_j^2)}{\zeta} \tag{1}
$$

Recall that
$$
\frac{d}{dx} \log(f(x)) = \frac{f'(x)}{f(x)}. \tag{2}
$$
We now have everything to compute the derivative
$$
\begin{aligned}
\frac{\partial \Omega}{\partial w_k} &= -\sum_i \frac{\partial}{\partial w_k} \log\left(\sum_j^M \pi_j \mathcal{N}(w_i | \mu_j, \sigma_j^2)\right) \\
&\overset{2}{=} -\sum_i \frac{\frac{\partial}{\partial w_k} \sum_{j = 1}^M \pi_j \mathcal{N}(w_i | \mu_j, \sigma_j^2)}{\zeta} \\
&= - \zeta^{-1} \sum_i \frac{\partial}{\partial w_k} \sum_{j = 1}^M \pi_j \mathcal{N}(w_i | \mu_j, \sigma_j^2) \\
&= - \zeta^{-1} \sum_i \sum_{j = 1}^M \pi_j \frac{\partial}{\partial w_k} \mathcal{N}(w_i | \mu_j, \sigma_j^2) \\
&= - \zeta^{-1} \sum_i \sum_{j = 1}^M \pi_j \frac{\partial}{\partial w_k} \frac{1}{\sqrt{2\pi\sigma_j^2}} \exp\left( - \frac{(w_i - \mu_j)^2}{2 \sigma_j^2}\right) \\
&= - \zeta^{-1} \sum_i \sum_{j = 1}^M \frac{\pi_j}{\sqrt{2\pi\sigma_j^2}} \frac{\partial}{\partial w_k} \exp\left( - \frac{(w_i - \mu_j)^2}{2 \sigma_j^2}\right)
\end{aligned}
$$
The expression
$$
\frac{\partial}{\partial w_k} \exp\left( - \frac{(w_i - \mu_j)^2}{2 \sigma_j^2}\right)
$$
is $0$ whenever $k \neq i$ and for $k = i$ we have
$$
\frac{\partial}{\partial w_i} \exp\left( - \frac{(w_i - \mu_j)^2}{2 \sigma_j^2}\right) = -\frac{w_i - \mu_j}{\sigma_j^2} \exp\left( - \frac{(w_i - \mu_j)^2}{2 \sigma_j^2}\right)
$$
Substituing this in the computation before yields
$$
\begin{aligned}
- \zeta^{-1} \sum_i \sum_{j = 1}^M \frac{\pi_j}{\sqrt{2\pi\sigma_j^2}} \frac{\partial}{\partial w_k} \exp\left( - \frac{(w_i - \mu_j)^2}{2 \sigma_j^2}\right) &= - \zeta^{-1} \sum_i \sum_{j = 1}^M \frac{\pi_j}{\sqrt{2\pi\sigma_j^2}} \left(-\frac{w_i - \mu_j}{\sigma_j^2} \exp\left( - \frac{(w_i - \mu_j)^2}{2 \sigma_j^2}\right)\right) \\
&= \zeta^{-1} \sum_i \sum_{j = 1}^M \frac{\pi_j}{\sqrt{2\pi\sigma_j^2}} \left(-\frac{w_i - \mu_j}{\sigma_j^2} \exp\left( \frac{(w_i - \mu_j)^2}{2 \sigma_j^2}\right)\right) \\
&= \zeta^{-1} \sum_i \sum_{j = 1}^M \pi_j \frac{1}{\sqrt{2\pi \sigma_j^2}} \exp\left(- \frac{(w_i - \mu_j)^2}{\sigma_j^2}\right) \frac{w_i - \mu_j}{\sigma_j^2} \\
&= \zeta^{-1} \sum_i \sum_{j = 1}^M \pi_j \mathcal{N}(w_i|\mu_j, \sigma_j^2) \frac{w_i - \mu_j}{\sigma_j^2} \\
&= \sum_i \sum_{j = 1}^M \frac{\pi_j \mathcal{N}(w_i|\mu_j, \sigma_j^2)}{\zeta} \frac{w_i - \mu_j}{\sigma_j^2} \\
&\overset{1}{=} \sum_i \sum_{j = 1}^M \gamma_j(w_i) \frac{w_i - \mu_j}{\sigma_j^2} \\
\end{aligned}
$$
With that we have shown that
$$
\frac{\partial \Omega}{\partial w_i} = \sum_j \gamma_j(w_i) \frac{w_i - \mu_j}{\sigma_j^2}
$$
and from that it immediately follows for
$$
\widetilde{E}(w) = E(w) + \lambda \Omega(w)
$$
that
$$
\frac{\partial \widetilde{E}}{\partial w_i} = \frac{\partial E}{\partial w_i} + \lambda \sum_j \gamma_j(w_i) \frac{w_i - \mu_j}{\sigma_j^2}
$$
which is what had to be shown.