# Exercise 5.8
We saw in (4.88) that the derivative of the logistic sigmoid activation function can be expressed in terms of the function value itself. Derive the corresponding result for the ‘tanh’ activation function deﬁned by (5.59).
$$
\sigma'(a) = \sigma(a)(1 - \sigma(a)) \tag{4.88}
$$
$$
\tanh(a) = \frac{e^a - e^{-a}}{e^a + e^{-a}}
$$

## Solution
Recall that
$$
\tanh(x) = 2 \sigma(2x) - 1 \tag{$*$}
$$
and equivalently
$$
\sigma(a) = \frac{1 + \tanh(a / 2)}{2}
$$
holds. From ($*$) we get
$$
\begin{aligned}
\tanh'(x) &= 4 \sigma'(2x) = 4 \sigma(2x)(1 - \sigma(2x)) \\
&\overset{*}{=} 4 \left(\frac{1 + \tanh(x)}{2}\right)\left(1 - \frac{1 + \tanh(x)}{2}\right) \\
&= (1 + \tanh(x))(1 - \tanh(x)) \\
&= 1 - \tanh^2(x).
\end{aligned}
$$